theories/Core/KTreeFacts.v
@@ -1,427 +1,291 @@
-(** * Theorems about the traced monoidal category of KTrees *)
-
-(** More precisely, facts about the trace operator [loop].
-    The coinductive reasoning is all done in [LoopFacts], and
-    this package just repackages it into nice categorical equations.
-
-    The monoidal category structure is verified in
-    [ITree.Core.KTreeBasicFacts].
- *)
+(** * Facts about [aloop] and [loop] *)
 
 (* begin hide *)
-Require Import Paco.paco.
-
 From Coq Require Import
-     Morphisms.
+     Program
+     Classes.Morphisms
+     Setoids.Setoid
+     Relations.Relations.
+
+From Paco Require Import paco.
 
 From ITree Require Import
      Basics.Basics
-     Basics.Category
+     Basics.CategoryOps
+     Basics.CategoryTheory
      Basics.Function
-     Basics.FunctionFacts
      Core.ITreeDefinition
      Core.KTree
      Eq.Eq
      Eq.UpToTaus.
 
-From ITree Require Export
-     Core.KTreeBasicFacts.
-
-From ITree Require Export
-     Core.LoopFacts.
-
 Import ITreeNotations.
 Import CatNotations.
-Local Open Scope itree_scope.
-Local Open Scope cat_scope.
+Local Open Scope itree.
 (* end hide *)
 
-(** *** Traced monoidal categories *)
+(** ** [ITree.aloop] *)
 
-Section TraceLaws.
-
-Local Opaque eqit loop ITree.bind'.
-
-Context {E : Type -> Type}.
-
-Local Open Scope cat.
-
-(** *** [loop] lemmas *)
-
-Global Instance eq_ktree_loop {I A B} :
-  Proper (eq2 ==> eq2) (@loop E I A B).
+Lemma bind_aloop {E A B C} (f : A -> itree E A + B) (g : B -> itree E B + C): forall x,
+    (ITree.aloop f x >>= ITree.aloop g)
+  ≈ ITree.aloop (fun ab =>
+       match ab with
+       | inl a => inl (ITree._aloop id (fun a => Ret (inl a))
+                                    (bimap (id_ _) inr (f a)))
+       | inr b => apply_Fun (bimap (ITree.map inr) (id_ _)) (g b)
+       end) (inl x).
 Proof.
-  repeat intro; apply eutt_loop; auto.
+  einit. ecofix CIH. intros.
+  rewrite !unfold_aloop. unfold ITree._aloop.
+  destruct (f x) as [t | b]; cbn.
+  - unfold id. rewrite bind_tau. etau. rewrite !bind_bind.
+    ebind. econstructor; try reflexivity.
+    intros. subst. rewrite bind_ret. eauto with paco.
+  - rewrite bind_ret, tau_eutt, bind_ret.
+    revert b. ecofix CIH'. intros.
+    rewrite !unfold_aloop. unfold ITree._aloop.
+    destruct (g b) as [t' | c]; cbn; eauto with paco.
+    rewrite bind_map. etau.
+    ebind. econstructor; try reflexivity.
+    intros. subst. eauto with paco.
 Qed.
 
-(* Naturality of (loop_ktree I A B) in A *)
-(* Or more diagrammatically:
-[[
-        +-----+
-        | ### |
-        +-###-+I
-A----B----###----C
-          ###
-
-is equivalent to:
-
-   +----------+
-   |      ### |
-   +------###-+I
-A----B----###----C
-          ###
-
-]]
- *)
-
-Lemma compose_loop {I A B C}
-      (bc_: ktree E (I + B) (I + C)) (ab: ktree E A B) :
-    loop (bimap (id_ _) ab >>> bc_)
-  ⩯ ab >>> loop bc_.
+Lemma eq_itree_aloop' {E I1 I2 R1 R2}
+      (RI : I1 -> I2 -> Prop)
+      (RR : R1 -> R2 -> Prop)
+      (body1 : I1 -> itree E I1 + R1)
+      (body2 : I2 -> itree E I2 + R2)
+      (eutt_body
+       : forall j1 j2, RI j1 j2 -> sum_rel (eq_itree RI) RR (body1 j1) (body2 j2))
+  : forall (i1 : I1) (i2 : I2) (RI_i : RI i1 i2),
+    @eq_itree E _ _ RR (ITree.aloop body1 i1) (ITree.aloop body2 i2).
 Proof.
-  intros a. cbv.
-  rewrite bind_loop2.
-  apply eutt_loop.
-  clear a.
-  intros [i | a']; cbn.
+  ginit. gcofix CIH. intros.
+  specialize (eutt_body i1 i2 RI_i).
+  do 2 rewrite unfold_aloop.
+  destruct eutt_body; cbn; eauto with paco.
+  gstep. econstructor. guclo eqit_clo_bind.
+  gstep. constructor; eauto.
+Qed.
+
+Lemma eutt_aloop' {E I1 I2 R1 R2}
+      (RI : I1 -> I2 -> Prop)
+      (RR : R1 -> R2 -> Prop)
+      (body1 : I1 -> itree E I1 + R1)
+      (body2 : I2 -> itree E I2 + R2)
+      (eutt_body
+       : forall j1 j2, RI j1 j2 -> sum_rel (eutt RI) RR (body1 j1) (body2 j2))
+  : forall (i1 : I1) (i2 : I2) (RI_i : RI i1 i2),
+    @eutt E _ _ RR (ITree.aloop body1 i1) (ITree.aloop body2 i2).
+Proof.
+  einit. ecofix CIH. intros.
+  specialize (eutt_body i1 i2 RI_i).
+  do 2 rewrite unfold_aloop.
+  destruct eutt_body; cbn; eauto with paco.
+  etau. ebind. econstructor; eauto with paco.
+Qed.
+
+(** ** [iter] *)
+
+Instance eq_itree_iter {E A B} :
+  @Proper ((A -> itree E (A + B)) -> A -> itree E B)
+          ((eq ==> eq_itree eq) ==> pointwise_relation _ (eq_itree eq))
+          iter.
+Proof.
+  intros body1 body2 EQ_BODY a. repeat red in EQ_BODY.
+  unfold iter, Iter_ktree.
+  eapply (eq_itree_aloop' eq).
+  intros [] ? []; constructor; auto. reflexivity.
+Qed.
+
+Instance eutt_iter {E A B} :
+  @Proper ((A -> itree E (A + B)) -> A -> itree E B)
+          (pointwise_relation _ (eutt eq) ==> pointwise_relation _ (eutt eq))
+          iter.
+Proof.
+  intros body1 body2 EQ_BODY a. repeat red in EQ_BODY.
+  unfold iter, Iter_ktree.
+  eapply (eutt_aloop' eq).
+  intros [] ? []; constructor; auto. reflexivity.
+Qed.
+
+Instance eq2_ktree_iter {E A B} :
+  @Proper (ktree E A (A + B) -> ktree E A B)
+          (eq2 ==> eq2)
+          iter.
+Proof. apply eutt_iter. Qed.
+
+Section KTreeConway.
+
+Lemma unfold_iter_ktree {E A B} (f : ktree E A (A + B)) (a0 : A) :
+  iter f a0 ≅ Tau (
+    ab <- f a0 ;;
+    match ab with
+    | inl a => iter f a
+    | inr b => Ret b
+    end).
+Proof.
+  unfold iter, Iter_ktree, cat, Cat_ktree, ITree.cat.
+  rewrite unfold_aloop; cbn.
+  pstep; constructor; left.
+  eapply eqit_bind; try reflexivity.
+  intros [].
+  reflexivity.
+  rewrite unfold_aloop; cbn.
+  reflexivity.
+Qed.
+
+Instance IterUnfold_ktree {E} : IterUnfold (ktree E) sum.
+Proof.
+  repeat intro.
+  rewrite unfold_iter_ktree, tau_eutt.
+  reflexivity.
+Qed.
+
+Instance IterNatural_ktree {E} : IterNatural (ktree E) sum.
+Proof.
+  repeat intro.
+  unfold bimap, Bimap_Coproduct, case_, Case_ktree, case_sum, cat, Cat_ktree, ITree.cat.
+  revert a0.
+  einit. ecofix CIH. intros.
+  rewrite 2 unfold_iter_ktree.
+  rewrite bind_tau.
+  estep; econstructor.
+  rewrite !bind_bind.
+  ebind; econstructor; try reflexivity.
+  intros [] ? [].
+  unfold id_, Id_ktree, inl_, Inl_ktree, lift_ktree.
+  rewrite 2 bind_ret.
+  eauto with paco.
+  rewrite bind_bind.
+  unfold inr_, Inr_ktree, lift_ktree.
+  setoid_rewrite bind_ret.
+  rewrite bind_ret2.
+  reflexivity.
+Qed.
+
+Lemma iter_dinatural_ktree {E A B C}
+      (f : ktree E A (C + B)) (g : ktree E C (A + B)) (a0 : A)
+  : iter (fun a =>
+      cb <- f a ;;
+      match cb with
+      | inl c => Tau (g c)
+      | inr b => Ret (inr b)
+      end) a0
+  ≅ Tau (
+       cb <- f a0 ;;
+       match cb with
+       | inl c0 => iter (fun c =>
+         ab <- g c ;;
+         match ab with
+         | inl a => Tau (f a)
+         | inr b => Ret (inr b)
+         end) c0
+       | inr b => Ret b
+       end).
+Proof.
+  revert A B C f g a0.
+  ginit. gcofix CIH. intros.
+  rewrite unfold_iter_ktree.
+  gstep; econstructor.
+  rewrite bind_bind.
+  guclo eqit_clo_bind. econstructor. try reflexivity.
+  intros [] ? [].
+  { rewrite bind_tau.
+    (* TODO: here we should be able to apply symmetry and be done. *)
+    rewrite unfold_iter_ktree.
+    gstep; econstructor.
+    rewrite bind_bind.
+    guclo eqit_clo_bind. econstructor. try reflexivity.
+    intros [] ? [].
+    { rewrite bind_tau.
+      eauto with paco.
+    }
+    { rewrite bind_ret. gstep; econstructor; auto.
+    }
+  }
+  { rewrite bind_ret. gstep; constructor; auto.
+  }
+Qed.
+
+Instance IterDinatural_ktree {E} : IterDinatural (ktree E) sum.
+Proof.
+  repeat intro.
+  unfold bimap, Bimap_Coproduct, case_, Case_ktree, case_sum, cat, Cat_ktree, ITree.cat.
+  transitivity (iter (fun t =>
+                        x <- f t;;
+                        match x with
+                        | inl a1 => Tau (g a1)
+                        | inr b0 => inr_ b0
+                        end) a0).
+  - apply eutt_iter; intros x.
+    eapply eutt_clo_bind.
+    reflexivity.
+    intros [] ? [].
+    rewrite tau_eutt; reflexivity.
+    reflexivity.
+  - rewrite iter_dinatural_ktree.
+    rewrite tau_eutt.
+    eapply eutt_clo_bind.
+    reflexivity.
+    intros [] ? [].
+    + apply eutt_iter; intros x.
+      eapply eutt_clo_bind.
+      reflexivity.
+      intros [] ? [].
+      rewrite tau_eutt; reflexivity.
+      reflexivity.
+    + reflexivity.
+Qed.
+
+Lemma iter_codiagonal_ktree {E A B} (f : ktree E A (A + (A + B))) (a0 : A)
+  : iter (iter f) a0
+  ≅ Tau (iter (fun a =>
+       r <- f a ;;
+       match r with
+       | inl a' => Ret (inl a')
+       | inr (inl a') => Tau (Ret (inl a'))
+       | inr (inr b) => Ret (inr b)
+       end) a0).
+Proof.
+  revert a0.
+  ginit. gcofix CIH. intros.
+  rewrite unfold_iter_ktree.
+  rewrite (unfold_iter_ktree (fun _ => _ _ _)).
+  gstep; constructor.
+  revert a0.
+  gcofix CIH'. intros.
+  rewrite bind_bind.
+  rewrite unfold_iter_ktree.
+  rewrite bind_tau, bind_bind.
+  gstep; constructor.
+  guclo eqit_clo_bind. econstructor. reflexivity.
+  intros [| []] ? [].
+  - rewrite bind_ret.
+    rewrite (unfold_iter_ktree (fun _ => _ _ _)).
+    auto with paco.
+  - rewrite bind_tau, 2 bind_ret.
+    auto with paco.
   - rewrite 2 bind_ret.
-    reflexivity.
-  - rewrite bind_bind. setoid_rewrite bind_ret.
-    reflexivity.
+    gstep; reflexivity.
 Qed.
 
-(* Naturality of (loop I A B) in B *)
-(* Or more diagrammatically:
-[[
-   +-----+
-   | ### |
-   +-###-+I
-A----###----B----C
-     ###
-
-is equivalent to:
-
-   +----------+
-   | ###      |
-   +-###------+I
-A----###----B----C
-     ###
-
-]]
- *)
-
-Lemma loop_compose {I A B B'}
-      (ab_: ktree E (I + A) (I + B)) (bc: ktree E B B') :
-    loop (ab_ >>> bimap (id_ _) bc)
-  ⩯ loop ab_ >>> bc.
+Instance IterCodiagonal_ktree {E} : IterCodiagonal (ktree E) sum.
 Proof.
-  intros a.
-  cbv.
-  rewrite bind_loop.
-  apply eutt_loop.
-  intros ia.
-  einit. ebind. econstructor; try reflexivity.
-  intros; subst. destruct u2.
-  - rewrite bind_ret; eauto with paco.
-  - reflexivity.
-Qed.
-
-(* Dinaturality of (loop I A B) in I *)
-
-Lemma loop_rename_internal {I J A B}
-      (ab_: ktree E (I + A) (J + B)) (ji: ktree E J I) :
-    loop (ab_ >>> bimap ji (id_ _))
-  ⩯ loop (bimap ji (id_ _) >>> ab_).
-Proof.
-  assert (trans4: forall r s t u : ktree E A B,
-             s ⩯ t -> r ⩯ s -> t ⩯ u -> r ⩯ u).
-  { intros.
-    do 2 (etransitivity; eauto). }
-  eapply trans4.
-  { intros a. erewrite (loop_bind ji ab_) at 1. reflexivity. }
-  { apply eutt_loop; cbv; intros ia.
-    einit. ebind. econstructor; try reflexivity.
-    intros; subst. destruct u2.
-    + rewrite tau_eutt. reflexivity.
-    + rewrite bind_ret. eauto with paco. }
-  { apply eutt_loop. cbv. intros [].
-    + einit. ebind. econstructor. 
-      * eapply eqit_bind; try reflexivity.
-        red; intros. rewrite tau_eutt. reflexivity.
-      * intros; subst. reflexivity.
-    + rewrite !bind_ret; reflexivity. }
-Qed.
-
-(* Loop over the empty set can be erased *)
-Lemma vanishing_ktree {A B: Type} (f: ktree E (void + A) (void + B)) :
-  loop f ⩯ unit_l' >>> f >>> unit_l.
-Proof.
-  intros a.
-  rewrite vanishing1_loop.
-  cbv.
-  rewrite bind_ret.
-  einit. ebind. econstructor; try reflexivity.
-  intros; subst. destruct u2; [contradiction|reflexivity]. 
-Qed.
-
-(* [loop_loop]:
-
-These two loops:
-
-[[
-    +----------+
-    | +-----+  |
-    | | ### |  |
-    | +-###-+I |
-    +---###----+J
-  A-----###-------B
-        ###
-]]
-
-... can be rewired as a single one:
-
-
-[[
-     +-------+
-     |  ###  |
-     +--###--+(I+J)
-     +--###--+
-  A-----###-----B
-        ###
-]]
-
- *)
-
-Lemma loop_loop {I J A B} (ab__: ktree E (I + (J + A)) (I + (J + B))) :
-    loop (loop ab__)
-  ⩯ loop (assoc_r >>> ab__ >>> assoc_l).
-Proof.
-  intros a.
-  rewrite vanishing2_loop.
-  cbv.
-  apply eutt_loop.
-  intros [[]|]; cbn.
-  all: rewrite !bind_bind.
-  all: try rewrite !bind_ret.
-  all: einit; ebind; econstructor; try reflexivity.
-  all: intros; subst; destruct u2; try rewrite bind_ret; try reflexivity.
-  all: destruct s; try rewrite bind_ret; reflexivity.
-Qed.
-
-Lemma fold_map {R S}:
-  forall (f: R -> S) (t: itree E R),
-    (x <- t;; Ret (f x)) ≅ (ITree.map f t).
-Proof.
-  intros; reflexivity.
-Qed.
-
-Local Transparent loop.
-
-Lemma bimap_ktree_loop {I A B C D}
-      (ab : ktree E (I + A) (I + B)) (cd : ktree E C D) :
-    bimap (loop ab) cd
-  ⩯ loop (assoc_l >>> bimap ab cd >>> assoc_r).
-Proof.
-  rewrite assoc_l_ktree, assoc_r_ktree.
-  rewrite lift_compose_ktree, compose_ktree_lift.
-  remember @loop as l; cbv.
-  intros []; subst l.
-  - rewrite fold_map.
-    rewrite (@superposing1_loop E A B I C D).
-    apply eutt_loop.
-    cbv; intros [|[]].
-    all: symmetry. (* protect the existential. *)
-    all: rewrite bind_bind.
-    all: setoid_rewrite bind_ret at 1.
-    all: reflexivity.
-  - unfold loop.
-    autorewrite with itree.
-    einit. ebind. econstructor; try reflexivity.
-    intros. subst.
-    autorewrite with itree.
-    rewrite unfold_aloop; cbn. reflexivity.
-Qed.
-
-(** Utility: lemma to ease working forward in an equational proof.
-      Make it more convenient to rewrite subterm only on one side of the equation.
- *)
-Fact fwd_eqn {a b : Type} (f g : ktree E a b) :
-  (forall h, h ⩯ f -> h ⩯ g) -> f ⩯ g.
-Proof.
-  intro H; apply H; reflexivity.
-Qed.
-
-(** Utility: lemmas to ease forward reasoning *)
-Fact cat_eq2_l {a b c : Type} (h : ktree E a b) (f g : ktree E b c) :
-  f ⩯ g ->
-  h >>> f ⩯ h >>> g.
-Proof.
-  intros H; rewrite H; reflexivity.
-Qed.
-
-Fact cat_eq2_r {a b c : Type} (h : ktree E b c) (f g : ktree E a b) :
-  f ⩯ g ->
-  f >>> h ⩯ g >>> h.
-Proof.
-  intros H; rewrite H; reflexivity.
-Qed.
-
-Fact local_rewrite1 {a b c : Type}:
-  bimap (id_ a) (@swap _ (ktree E) _ _ b c) >>> assoc_l >>> swap
-        ⩯ assoc_l >>> bimap swap (id_ c) >>> assoc_r.
-Proof.
-  symmetry.
-  apply fwd_eqn; intros h Eq.
-  do 2 apply (cat_eq2_l (bimap (id_ _) swap)) in Eq.
-  rewrite <- cat_assoc, bimap_cat, swap_involutive, cat_id_l,
-  bimap_id, cat_id_l in Eq.
-  rewrite <- (cat_assoc _ _ assoc_r), <- (cat_assoc _ assoc_l _)
-    in Eq.
-  rewrite <- swap_assoc_l in Eq.
-  rewrite (cat_assoc _ _ assoc_r) in Eq.
-  rewrite assoc_l_mono in Eq.
-  rewrite cat_id_r in Eq.
-  rewrite cat_assoc.
-  assumption.
-Qed.
-
-Fact local_rewrite2 {a b c : Type}:
-  swap >>> assoc_r >>> bimap (id_ _) swap
-       ⩯ @assoc_l _ (ktree E) _ _ a b c >>> bimap swap (id_ _) >>> assoc_r.
-Proof.
-  symmetry.
-  apply fwd_eqn; intros h Eq.
-  do 2 apply (cat_eq2_r (bimap (id_ _) swap)) in Eq.
-  rewrite cat_assoc, bimap_cat, swap_involutive, cat_id_l,
-  bimap_id, cat_id_r in Eq.
-  rewrite 2 (cat_assoc assoc_l) in Eq.
-  rewrite <- swap_assoc_r in Eq.
-  rewrite <- 2 (cat_assoc assoc_l) in Eq.
-  rewrite assoc_l_mono, cat_id_l in Eq.
-  assumption.
-Qed.
-
-Lemma loop_bimap_ktree {I A B C D}
-      (ab : ktree E A B) (cd : ktree E (I + C) (I + D)) :
-  bimap ab (loop cd)
-        ⩯ loop (assoc_l >>> bimap swap (id_ _)
-                        >>> assoc_r
-                        >>> bimap ab cd
-                        >>> assoc_l >>> bimap swap (id_ _) >>> assoc_r).
-Proof.
-  rewrite swap_bimap, bimap_ktree_loop.
-  rewrite <- compose_loop, <- loop_compose.
-  rewrite (swap_bimap cd ab).
-  rewrite <- !cat_assoc.
-  rewrite local_rewrite1.
-  rewrite 2 cat_assoc.
-  rewrite <- (cat_assoc swap assoc_r).
-  rewrite local_rewrite2.
-  rewrite <- !cat_assoc.
+  repeat intro.
+  unfold bimap, Bimap_Coproduct, case_, Case_ktree, case_sum, cat, Cat_ktree, ITree.cat.
+  rewrite iter_codiagonal_ktree.
+  rewrite tau_eutt.
+  apply eutt_iter.
+  intros a1.
+  eapply eutt_clo_bind.
   reflexivity.
+  intros [| []] ? []; rewrite ?tau_eutt; reflexivity.
 Qed.
 
-Lemma yanking_ktree {A: Type}:
-  @loop E _ _ _ swap ⩯ id_ A.
+Global Instance Conway_ktree {E} : Conway (ktree E) sum.
 Proof.
-  intros ?; rewrite yanking_loop. rewrite tau_eutt. reflexivity.
+  split; typeclasses eauto.
 Qed.
 
-Lemma loop_rename_internal' {I J A B} (ij : ktree E I J) (ji: ktree E J I)
-      (ab_: @ktree E (I + A) (I + B)) :
-  (ij >>> ji) ⩯ id_ _ ->
-    loop (bimap ji (id_ _) >>> ab_ >>> bimap ij (id_ _))
-  ⩯ loop ab_.
-Proof.
-  intros Hij.
-  rewrite loop_rename_internal.
-  rewrite <- cat_assoc.
-  rewrite bimap_cat.
-  rewrite Hij.
-  rewrite cat_id_l.
-  rewrite bimap_id.
-  rewrite cat_id_l.
-  reflexivity.
-Qed.
-
-End TraceLaws.
-
-Hint Rewrite @bimap_id_lift : lift_ktree.
-Hint Rewrite @bimap_lift_id : lift_ktree.
-Hint Rewrite @lift_case_sum : lift_ktree.
-
-(* Here we show that we can implement [ITree.cat] using
-   [bimap], [loop], and composition with the monoidal
-   natural isomorphisms. *)
-
-(* [cat_from_loop]:
-
-      +-------------+
-      |             |
-      +---\/---ab---+
-   -------/\---bc-------
-
-is equivalent to
-
-   ----ab---bc----
- *)
-Theorem cat_from_loop {E A B C} (ab : ktree E A B) (bc : ktree E B C) :
-  loop (swap >>> bimap ab bc) ⩯ ab >>> bc.
-Proof.
-(*
-      +-------------+
-      |             |
-      +---\/---ab---+
-   -------/\---bc-------
- *)
-
-  rewrite bimap_slide...
-  rewrite <- cat_assoc...
-(*
-      +----------------+
-      |                |
-      +---\/---ab------+
-   -------/\------bc-------
- *)
-
-  rewrite loop_compose...
-(*
-      +-------------+
-      |             |
-      +---\/---ab---+
-   -------/\------------bc----
- *)
-
-  rewrite swap_bimap...
-  rewrite <- !cat_assoc...
-(*
-      +-------------------+
-      |                   |
-      +---\/--\/------\/--+
-   -------/\--/\--ab--/\----bc----
- *)
-
-  rewrite swap_involutive, cat_id_l...
-(*
-      +-------------------+
-      |                   |
-      +---------------\/--+
-   ---------------ab--/\----bc----
- *)
-
-  rewrite compose_loop...
-(*
-           +------+
-           |      |
-           +--\/--+
-   ----ab-----/\-----bc----
- *)
-
-  rewrite yanking_ktree...
-  rewrite cat_id_r...
-(*
-   ----ab---bc----
- *)
-
-  reflexivity.
-Qed.
+End KTreeConway.
