theories/Interp/InterpFacts.v
@@ -20,6 +20,7 @@ From ITree Require Import
      Basics.Basics
      Core.ITreeDefinition
      Core.KTree
+     Core.KTreeFacts
      Eq.Eq
      Eq.UpToTaus
      Indexed.Sum
@@ -307,13 +308,36 @@ Proof.
   - rewrite interp_ret. gstep. constructor; auto.
 Qed.
 
+Lemma interp_iter {E F} (f : E ~> itree F) {A B}
+      (t : A -> itree E (A + B)) a0
+  : interp f (iter t a0) ≅ iter (fun a => interp f (t a)) a0.
+Proof.
+  unfold iter, Iter_ktree.
+  apply interp_aloop.
+  intros []; constructor; reflexivity.
+Qed.
+
 Lemma interp_loop {E F} (f : E ~> itree F) {A B C}
       (t : C + A -> itree E (C + B)) a :
   interp f (loop t a) ≅ loop (fun ca => interp f (t ca)) a.
 Proof.
-  unfold loop.
+  unfold loop. unfold cat, Cat_ktree, ITree.cat.
+  rewrite interp_bind.
+  apply eqit_bind.
+  repeat intro.
+  rewrite interp_iter.
+  apply eq_itree_iter.
+  intros ? ? [].
   rewrite interp_bind.
   apply eqit_bind; try reflexivity.
-  red. apply interp_aloop.
-  intros []; cbn; constructor; reflexivity.
+  intros []; cbn. unfold cat. rewrite interp_bind.
+  unfold inl_, Inl_ktree, inr_, Inr_ktree, lift_ktree.
+  rewrite interp_ret, !bind_ret, interp_ret.
+  reflexivity.
+  unfold cat, id_, Id_ktree, inr_, Inr_ktree, lift_ktree.
+  rewrite interp_bind, interp_ret, !bind_ret, interp_ret.
+  reflexivity.
+  unfold inr_, Inr_ktree, lift_ktree.
+  rewrite interp_ret.
+  reflexivity.
 Qed.
